try spilling proof with normal separation logic on locals map

compiler/src/compiler/Spilling.v
@@ -18,177 +18,140 @@ Require Import bedrock2.MetricLogging.
 
 Open Scope Z_scope.
 
+Ltac specialize_rec H :=
+  lazymatch type of H with
+  | ?P -> ?Q => let F := fresh in assert P as F; [clear H|specialize (H F); clear F; specialize_rec H]
+  | forall (x: ?T), _ => let n := fresh x in evar (n: T); specialize (H n); subst n; specialize_rec H
+  | _ => idtac
+  end.
+
+Tactic Notation "spec" constr(t) "as" ident(H) := pose proof t as H; specialize_rec H.
+
+Lemma sumbool_of_BoolSpec: forall {P Q: Prop} {b: bool},
+    BoolSpec P Q b -> {P} + {Q}.
+Proof.
+  intros. destruct b.
+  - left. inversion H. assumption.
+  - right. inversion H. assumption.
+Defined.
+
+Lemma sumbool_of_EqDecider{T: Type}{d: T -> T -> bool}:
+  EqDecider d ->
+  forall x y: T, {x = y} + {x <> y}.
+Proof. intros. eapply sumbool_of_BoolSpec. apply H. Qed.
+
 Module map.
   Section MAP.
     Context {key value} {map : map.map key value}.
-
-    Definition dom(l: map): key -> Prop := fun x => exists v, map.get l x = Some v.
-
-    Inductive mut_disj: list map -> Prop :=
-    | mut_disj_nil:
-        mut_disj []
-    | mut_disj_cons: forall m l,
-        (forall m', In m' l -> map.disjoint m m') ->
-        mut_disj l ->
-        mut_disj (m :: l).
-
-    Definition map_keys{key': Type}{map': map.map key' value}(f: key -> key'): map -> map' :=
-      map.fold (fun m' k v => map.put m' (f k) v) map.empty.
-
-    Definition join: list map -> map := List.fold_right map.putmany map.empty.
-
-    Definition splits(L R: list map): Prop := join L = join R /\ mut_disj L /\ mut_disj R.
-
-    Definition geto(a: option map)(k: key): option value :=
-      match a with
-      | Some m => map.get m k
-      | None => None
-      end.
-
-    Definition domo(a: option map): key -> Prop :=
-      match a with
-      | Some m => fun k => exists v, map.get m k = Some v
-      | None => fun k => True (* TODO depending on where it's used, this should be False *)
-      end.
-
-    Definition putmanyo(a b: option map): option map :=
-      match a, b with
-      | Some a, Some b => Some (map.putmany a b)
-      | _, _ => None
-      end.
-
-    (* domains need not be disjoint, but if they overlap, the two maps have to agree on the value *)
-    Definition agreeing_putmany{value_eqb: value -> value -> bool}{value_eq_spec: EqDecider value_eqb}
-               (a b: option map): option map :=
-      match a, b with
-      | Some a, Some b => map.fold (fun o k v => match o with
-                                                 | Some m => match map.get m k with
-                                                             | Some v' => if value_eqb v v'
-                                                                          then Some m else None
-                                                             | None => Some (map.put m k v)
-                                                             end
-                                                 | None => None
-                                                 end)
-                                   (Some a)
-                                   b
-      | _, _ => None
-      end.
-
-    Definition disj_putmany(a b: option map): option map :=
-      match a, b with
-      | Some a, Some b => map.fold (fun o k v => match o with
-                                                 | Some m => match map.get m k with
-                                                             | Some _ => None
-                                                             | None => Some (map.put m k v)
-                                                             end
-                                                 | None => None
-                                                 end)
-                                   (Some a)
-                                   b
-      | _, _ => None
-      end.
-
-    Lemma disj_putmany_empty_l: forall m: option map,
-        disj_putmany (Some map.empty) m = m.
-    Admitted.
-
-    Lemma disj_putmany_empty_r: forall m: option map,
-        disj_putmany m (Some map.empty) = m.
-    Admitted.
-
     Context {ok : map.ok map} {key_eqb: key -> key -> bool} {key_eq_dec : EqDecider key_eqb}.
 
-    Lemma mut_disj_disjoint: forall m1 m2,
-        mut_disj [m1; m2] ->
-        map.disjoint m1 m2.
+    (* to get stronger guarantees such as indexing into vs, we'd need NoDup *)
+    Lemma putmany_of_list_zip_get: forall (ks: list key) (vs: list value) m0 m k,
+        map.putmany_of_list_zip ks vs m0 = Some m ->
+        In k ks ->
+        map.get m k <> None.
     Proof.
-      intros. inversion H. subst. eapply H2. simpl. auto.
+      induction ks as [|k ks]; intros.
+      - simpl in H0. destruct H0.
+      - simpl in H0. destruct H0.
+        + subst k0. cbn in H. simp. intro C.
+          eapply map.putmany_of_list_zip_to_putmany in H.
+          destruct H as (M & A & B). subst m.
+          rewrite map.get_putmany_dec in C. rewrite map.get_put_same in C.
+          destruct_one_match_hyp; discriminate.
+        + cbn in H. simp. eapply IHks; eauto.
     Qed.
 
-    Lemma disjoint_mut_disj: forall m1 m2,
-        map.disjoint m1 m2 ->
-        mut_disj [m1; m2].
-    Proof.
-      intros. repeat constructor; simpl; intros; subst; try contradiction.
-      destruct H0; subst; try assumption. contradiction.
-    Qed.
-
-    Lemma split_splits: forall m m1 m2,
+    Lemma split_remove_put: forall m m1 m2 k v,
         map.split m m1 m2 ->
-        splits [m] [m1; m2].
+        map.get m k = Some v ->
+        map.split m (map.remove m1 k) (map.put m2 k v).
     Proof.
-      unfold map.split, splits, join. simpl. intros. destruct H. subst. split.
-      - rewrite ?map.putmany_empty_r. reflexivity.
-      - repeat constructor; simpl; intros; try contradiction.
-        destruct H; subst; firstorder idtac.
+      intros.
+      destruct (map.get_split k _ _ _ H) as [(A & B) | (A & B)].
+      - eapply map.split_put_l2r.
+        + apply map.get_remove_same.
+        + replace (map.put (map.remove m1 k) k v) with m1. 1: assumption.
+          apply map.map_ext.
+          intro x.
+          rewrite map.get_put_dec.
+          destruct_one_match.
+          * subst x. congruence.
+          * rewrite map.get_remove_diff by congruence. reflexivity.
+      - replace (map.remove m1 k) with m1. 2: {
+          eapply map.map_ext. intro x. rewrite map.get_remove_dec.
+          destruct_one_match.
+          - subst x. assumption.
+          - reflexivity.
+        }
+        replace (map.put m2 k v) with m2. 2: {
+          apply map.map_ext. intro x. rewrite map.get_put_dec.
+          destruct_one_match.
+          - subst x. congruence.
+          - reflexivity.
+        }
+        assumption.
     Qed.
 
-    Lemma splits_split: forall m m1 m2,
-        splits [m] [m1; m2] ->
-        map.split m m1 m2.
+    Lemma getmany_of_list_to_split: forall m (ks: list key) (vs: list value),
+        map.getmany_of_list m ks = Some vs ->
+        exists mrest mks, map.of_list_zip ks vs = Some mks /\ map.split m mrest mks.
     Proof.
-      unfold map.split, splits, join. simpl. intros. destruct H as (?&?&?).
-      apply mut_disj_disjoint in H1.
-      rewrite ?map.putmany_empty_r in H.
-      auto.
+      induction ks as [|k ks]; intros; destruct vs as [|v vs].
+      - do 2 eexists. split. 1: reflexivity. unfold map.split. rewrite map.putmany_empty_r.
+        split. 1: reflexivity. apply map.disjoint_empty_r.
+      - discriminate.
+      - cbn in H. simp. destruct_one_match_hyp; discriminate.
+      - cbn in H. simp. specialize (IHks _ E0). simp. cbn.
+        unfold map.of_list_zip in *.
+        exists (map.remove mrest k), (map.put mks k v). split.
+        + destr (map.putmany_of_list_zip ks vs (map.put map.empty k v)). 2: {
+            pose proof map.putmany_of_list_zip_sameLength _ _ _ _ IHksp0 as C.
+            eapply map.sameLength_putmany_of_list in C. destruct C as [a C].
+            rewrite E1 in C. discriminate.
+          }
+          f_equal.
+          eapply map.map_ext.
+          intro x.
+          eapply map.putmany_of_list_zip_to_putmany in E1.
+          destruct E1 as (mks' & F & G).
+          subst r.
+          rewrite IHksp0 in F. apply Option.eq_of_eq_Some in F. subst mks'.
+          rewrite map.get_putmany_dec.
+          rewrite !map.get_put_dec.
+          rewrite map.get_empty.
+          destr (key_eqb k x). 2: destruct_one_match; reflexivity.
+          subst x.
+          destruct_one_match. 2: reflexivity.
+          unfold map.split in IHksp1. simp.
+          rewrite map.get_putmany_dec in E.
+          rewrite E1 in E.
+          assumption.
+        + eapply split_remove_put; assumption.
     Qed.
-
-    Axiom split_spec: forall (M A B: map),
-        map.split M A B <-> forall k,
-          (exists v, map.get M k = Some v /\
-                     ((map.get A k = Some v /\ map.get B k = None) \/
-                      (map.get B k = Some v /\ map.get A k = None))) \/
-          (map.get M k = None /\ map.get A k = None /\ map.get B k = None).
-
-    Axiom putmany_spec: forall (m1 m2: map) k,
-        (exists v, map.get (map.putmany m1 m2) k = Some v /\
-                   (map.get m2 k = Some v \/ (map.get m2 k = None /\ map.get m1 k = Some v))) \/
-        (map.get (map.putmany m1 m2) k = None /\ map.get m2 k = None /\ map.get m1 k = None).
-
-    Axiom getmany_of_list_shrink: forall (l l1 l2: map) keys,
-        map.split l l1 l2 ->
-        Forall (fun k => map.get l2 k = None) keys ->
-        map.getmany_of_list l keys = map.getmany_of_list l1 keys.
-
-    Axiom putmany_of_list_zip_split: forall (l l' l1 l2: map) keys values,
-        map.putmany_of_list_zip keys values l = Some l' ->
-        map.split l l1 l2 ->
-        Forall (fun k => map.get l2 k = None) keys ->
-        exists l1', map.split l' l1' l2 /\ map.putmany_of_list_zip keys values l1 = Some l1'.
-
-    Axiom putmany_of_list_zip_grow: forall (l l1 l1' l2: map) keys values,
-        map.putmany_of_list_zip keys values l1 = Some l1' ->
-        map.split l l1 l2 ->
-        Forall (fun k => map.get l2 k = None) keys ->
-        exists l', map.split l' l1' l2 /\ map.putmany_of_list_zip keys values l = Some l'.
-
-    Lemma getmany_of_list_preserved: forall (l1 l2: map) ks,
-        (forall k, In k ks -> map.get l1 k = map.get l2 k) ->
-        map.getmany_of_list l1 ks = map.getmany_of_list l2 ks.
-    Proof.
-      induction ks; intros. 1: reflexivity.
-      unfold map.getmany_of_list in *. simpl.
-      rewrite IHks. 2: {
-        intros. eapply H. simpl. auto.
-      }
-      specialize (H a). simpl in H. rewrite H. 2: auto.
-      reflexivity.
-    Qed.
-
-    (* disjoint-unions *)
-    Definition dus'(l: list (option map)): option map :=
-      List.fold_left (fun res e => disj_putmany res e) l (Some map.empty).
-
-    Fixpoint dus (xs : list (option map)) : option map :=
-      match xs with
-      | [x] => x
-      | x :: xs => disj_putmany (dus xs) x
-      | nil => Some map.empty
-      end.
-
   End MAP.
 End map.
 
+Section MoreSepLog.
+  Context {key value} {map : map.map key value}.
+  Context {ok : map.ok map} {key_eqb: key -> key -> bool} {key_eq_dec : EqDecider key_eqb}.
+
+  Lemma subst_split: forall (m m1 m2 M: map) (R: map -> Prop),
+      map.split m m1 m2 ->
+      (eq m * R)%sep M ->
+      (eq m1 * eq m2 * R)%sep M.
+  Proof.
+    (* FIRSTORDER? *)
+    intros.
+    unfold map.split in H. simp.
+    use_sep_assumption.
+    cancel.
+    cbn [seps].
+    intro m. unfold sep, map.split. split; intros.
+    - subst. eauto 10.
+    - simp. reflexivity.
+  Qed.
+End MoreSepLog.
 
 Section Spilling.
 
@@ -383,102 +346,18 @@ Section Spilling.
       intuition try blia.
   Qed.
 
-  Definition oeq{T: Type}(oL oR: option T): Prop := exists L R, oL = Some L /\ oR = Some R /\ oL = oR.
-
-  Notation "a \+/ b" := (map.disj_putmany a b) (at level 34, left associativity).
-  Notation "a \</ b" := (map.putmanyo a b) (at level 34, left associativity).
-  Notation "a \?/ b" := (map.agreeing_putmany a b) (at level 34, left associativity).
-  Notation "k ~> v" := (Some (map.put map.empty k v)) (at level 30).
-
-  Infix "==" := oeq (at level 38).
-
-  Definition one(sz: Syntax.access_size.access_size)(addr value: word): option mem :=
-    Some (map.putmany_of_tuple (Memory.footprint addr (@Memory.bytes_per width sz))
-                               (LittleEndian.split (@Memory.bytes_per width sz) (word.unsigned value))
-                               map.empty).
-
-  Definition array{T: Type}(elem: word -> T -> option mem)(size: word): word -> list T -> option mem :=
-    fix rec addr ls :=
-      match ls with
-      | [] => Some map.empty
-      | e :: es => elem addr e \+/ rec (word.add addr size) es
-      end.
-
-  Definition word_array: word -> list word -> option mem :=
-    array (one Syntax.access_size.word) (word.of_Z bytes_per_word).
-
-  Definition related(maxvar: Z)(frame: option mem)(done: bool)
-             (t1: trace)(m1: option mem)(l1: option locals)(mc1: MetricLog)
-             (t2: trace)(m2: option mem)(l2: option locals)(mc2: MetricLog): Prop :=
+  Definition related(maxvar: Z)(frame: mem -> Prop)(done: bool)
+             (t1: trace)(m1: mem)(l1: locals)(mc1: MetricLog)
+             (t2: trace)(m2: mem)(l2: locals)(mc2: MetricLog): Prop :=
       exists fpval tmp1val tmp2val lStack lRegs stackwords,
         t1 = t2 /\
-        m2 == m1 \+/ word_array fpval stackwords \+/ frame /\
-        subset (map.domo lRegs) (fun x => fp < x < 32) /\
-        subset (map.domo lStack) (fun x => 32 <= x <= maxvar) /\
-        l1 = lRegs \+/ lStack /\
-        l2 = lRegs \+/ tmp1 ~> tmp1val \+/ tmp2 ~> tmp2val \+/ fp ~> fpval /\
-        forall r, 32 <= r <= maxvar -> forall v, map.geto lStack r = Some v ->
+        (eq m1 * word_array fpval stackwords * frame)%sep m2 /\
+        (forall x v, map.get lRegs x = Some v -> fp < x < 32) /\
+        (forall x v, map.get lStack x = Some v -> 32 <= x <= maxvar) /\
+        (eq lRegs * eq lStack)%sep l1 /\
+        (eq lRegs * ptsto tmp1 tmp1val * ptsto tmp2 tmp2val * ptsto fp fpval)%sep l2 /\
+        forall r, 32 <= r <= maxvar -> forall v, map.get lStack r = Some v ->
            nth_error stackwords (Z.to_nat (r - 32)) = Some v.
-
-  (*
-  Notation "m [ k := v ]" := (map.put m k v) (at level 10, left associativity, format "m [ k  :=  v ]").
-  Notation "m [ k ]" := (map.get m k) (at level 10, left associativity, format "m [ k ]").
-  (* this notation overrides the notation for applying a function m to the singleton list containing k,
-     but that's so rare that it's fine *)
-
-  Definition related(maxvar: Z)(frame: mem)(done: bool):
-    FlatImp.SimState Z -> FlatImp.SimState Z -> Prop :=
-    fun '(t1, m1, l1, mc1) '(t2, m2, l2, mc2) =>
-      exists fpval tmp1val tmp2val mStack lStack lRegs,
-        t1 = t2 /\
-        m2 = map.putmany m1 (map.putmany mStack frame) /\
-        disjoint (map.dom m1) (map.dom mStack) /\
-        disjoint (map.dom m1) (map.dom frame) /\
-        disjoint (map.dom mStack) (map.dom frame) /\
-        subset (map.dom lRegs) (fun x => fp < x < 32) /\
-        subset (map.dom lStack) (fun x => 32 <= x <= maxvar) /\
-        l1 = map.putmany lRegs lStack /\
-        l2 = lRegs[tmp1 := tmp1val][tmp2 := tmp2val][fp := fpval] /\
-        spilled_vars fpval maxvar lStack mStack.
-
-  Definition related(maxvar: Z)(frame: option mem)(done: bool)
-             (t1: trace)(m1: option mem)(l1: option locals)(mc1: MetricLog)
-             (t2: trace)(m2: option mem)(l2: option locals)(mc2: MetricLog): Prop :=
-      exists fpval tmp1val tmp2val mStack lStack lRegs,
-        t1 = t2 /\
-        m2 = m1 \+/ mStack \+/ frame /\
-        subset (map.domo lRegs) (fun x => fp < x < 32) /\
-        subset (map.domo lStack) (fun x => 32 <= x <= maxvar) /\
-        l1 = lRegs \+/ lStack /\
-        l2 = lRegs \+/ tmp1 ~> tmp1val \+/ tmp2 ~> tmp2val \+/ fp ~> fpval /\
-        spilled_vars fpval maxvar lStack mStack.
-
-  Definition related(maxvar: Z)(frame: mem)(done: bool):
-    FlatImp.SimState Z -> FlatImp.SimState Z -> Prop :=
-    fun '(t1, m1, l1, mc1) '(t2, m2, l2, mc2) =>
-      exists fpval tmp1val tmp2val mStack lStack lRegs,
-        t1 = t2 /\
-        Some m2 = Some m1 \+/ Some mStack \+/ Some frame /\
-        subset (map.dom lRegs) (fun x => fp < x < 32) /\
-        subset (map.dom lStack) (fun x => 32 <= x <= maxvar) /\
-        Some l1 = Some lRegs \+/ Some lStack /\
-        Some l2 = Some lRegs \+/ tmp1 ~> tmp1val \+/ tmp2 ~> tmp2val \+/ fp ~> fpval /\
-        spilled_vars fpval maxvar lStack mStack.
-
-  Notation "k ~> v" := (map.put map.empty k v) (at level 30).
-
-  Definition related(maxvar: Z)(frame: mem)(done: bool):
-    FlatImp.SimState Z -> FlatImp.SimState Z -> Prop :=
-    fun '(t1, m1, l1, mc1) '(t2, m2, l2, mc2) =>
-      exists fpval tmp1val tmp2val mStack lStack lRegs,
-        t1 = t2 /\
-        map.splits [m2] [m1; mStack; frame] /\
-        subset (map.dom lRegs) (fun x => fp < x < 32) /\
-        subset (map.dom lStack) (fun x => 32 <= x <= maxvar) /\
-        map.splits [l1] [lRegs; lStack] /\
-        map.splits [l2] [lRegs; tmp1 ~> tmp1val; tmp2 ~> tmp2val; fp ~> fpval] /\
-        spilled_vars fpval maxvar lStack mStack.
-*)
 
   Definition envs_related(e1 e2: env): Prop :=
     forall f argvars resvars body1,
@@ -492,320 +371,50 @@ Section Spilling.
     intros. eapply exec.seq. 1: eassumption. simpl. clear. auto.
   Qed.
 
-  Lemma load_putmany_l: forall m1 m2 sz a v,
-      Memory.load sz m1 a = Some v ->
-      disjoint (map.dom m1) (map.dom m2) ->
-      Memory.load sz (map.putmany m1 m2) a = Some v.
-  Proof.
-  Admitted.
-
-  (* cps style
-  Lemma load_arg_reg1_correct: forall e a t m l mc post,
-      post ... ->
-      exec e (load_arg_reg1 a) t m l mc post. *)
-
-  (* seq style
-  Lemma load_arg_reg1_correct: forall e s a t m l mc post,
-      exec e s t
-      exec e (SSeq (load_arg_reg1 a) s) t m l mc post. *)
-
-  Arguments map.disj_putmany : simpl never.
-
-  Implicit Types post : trace -> option mem -> option locals -> MetricLog -> Prop.
-
-  Section WithE.
-    Variable (e: env).
-
-(*
-    Definition ext_spec' t mGive action argvals (outcome: mem -> list word -> Prop) :=
-      match mGive with
-      | Some mGive => ext_spec t mGive action argvals outcome
-      | None => False
-      end.
-
-    Definition ext_spec' t mGive action argvals (outcome: option mem -> list word -> Prop) :=
-      match mGive with
-      | Some mGive => ext_spec t mGive action argvals
-                               (fun mReceive resvals => outcome (Some mReceive) resvals)
-      | None => False
-      end.
-*)
-
-    Inductive exec:
-      stmt ->
-      trace -> option mem -> option locals -> MetricLog ->
-      (trace -> option mem -> option locals -> MetricLog -> Prop)
-    -> Prop :=
-    | interact: forall t m mKeep mGive l l_not_read l_not_written oldresvals mc action argvars
-                       argvals resvars outcome post,
-        m == mKeep \+/ Some mGive ->
-        l == l_not_read \+/ map.of_list_zip argvars argvals ->
-        l == l_not_written \+/ map.of_list_zip resvars oldresvals ->
-        ext_spec t mGive action argvals outcome ->
-        (forall mReceive resvals,
-            outcome mReceive resvals ->
-            exists l', l' == l_not_written \+/ map.of_list_zip resvars resvals /\
-            forall m', m' == mKeep \+/ Some mReceive ->
-            post (((mGive, action, argvals), (mReceive, resvals)) :: t) m' l'
-                 (addMetricInstructions 1
-                 (addMetricStores 1
-                 (addMetricLoads 2 mc)))) ->
-        exec (SInteract resvars action argvars) t m l mc post
-
-    | call: forall t m l mc binds fname args params rets fbody (*argvs st0*) post (* outcome *),
-        map.get e fname = Some (params, rets, fbody) ->
-        (* TODO
-        map.getmany_of_list l args = Some argvs ->
-        map.putmany_of_list_zip params argvs map.empty = Some st0 ->
-        exec fbody t m st0 mc outcome ->
-        (forall t' m' mc' st1,
-            outcome t' m' st1 mc' ->
-            exists retvs l',
-              map.getmany_of_list st1 rets = Some retvs /\
-              map.putmany_of_list_zip binds retvs l = Some l' /\
-              post t' m' l' mc') ->
-              *)
-        exec (SCall binds fname args) t m l mc post
-    | load: forall t m mFrame l l' lFrame mc sz x a o v addr post,
-        l == lFrame \+/ a ~> addr ->
-        m == mFrame \+/ one sz (word.add addr (word.of_Z o)) v ->
-        l' == l \</ x ~> v ->
-        post t m l'
-             (addMetricLoads 2
-             (addMetricInstructions 1 mc)) ->
-        exec (SLoad sz x a o) t m l mc post
-    | store: forall t (m mFrame m': option mem) mc l lFrame sz a o addr v (val oldval: word) post,
-        l == lFrame \+/ (a ~> addr \?/ v ~> val) ->
-        m == mFrame \+/ one sz (word.add addr (word.of_Z o)) oldval ->
-        m' == mFrame \+/ one sz (word.add addr (word.of_Z o)) val ->
-        post t m' l
-             (addMetricLoads 1
-             (addMetricInstructions 1
-             (addMetricStores 1 mc))) ->
-        exec (SStore sz a v o) t m l mc post
-    | stackalloc: forall t mSmall l mc x n body post,
-        n mod bytes_per_word = 0 ->
-        (forall l0 a stacktrash mCombined,
-            mCombined == mSmall \+/ map.of_disjoint_list_zip (Memory.ftprint a n) stacktrash ->
-            l0 == l \</ x ~> a ->
-            exec body t mCombined l0 (addMetricLoads 1 (addMetricInstructions 1 mc))
-             (fun t' mCombined' l' mc' =>
-              exists mSmall' stacktrash',
-                mCombined' == mSmall' \+/ map.of_disjoint_list_zip (Memory.ftprint a n) stacktrash' /\
-                post t' mSmall' l' mc')) ->
-        exec (SStackalloc x n body) t mSmall l mc post
-
-(*
-    | lit: forall t m l mc x v post,
-        post t m (map.put l x (word.of_Z v))
-             (addMetricLoads 8
-             (addMetricInstructions 8 mc)) ->
-        exec (SLit x v) t m l mc post
-*)
-
-    | op: forall t m l l' lFrame mc x op y y' z z' post,
-        l == lFrame \+/ (y ~> y' \?/ z ~> z') ->
-        l' == l \</ x ~> Semantics.interp_binop op y' z' ->
-        post t m l'
-             (addMetricLoads 2
-             (addMetricInstructions 2 mc)) ->
-        exec (SOp x op y z) t m l mc post
-
-(*
-    | set: forall t m l mc x y y' post,
-        map.get l y = Some y' ->
-        post t m (map.put l x y')
-             (addMetricLoads 1
-             (addMetricInstructions 1 mc)) ->
-        exec (SSet x y) t m l mc post
-    | if_true: forall t m l mc cond  bThen bElse post,
-        eval_bcond l cond = Some true ->
-        exec bThen t m l
-             (addMetricLoads 2
-             (addMetricInstructions 2
-             (addMetricJumps 1 mc))) post ->
-        exec (SIf cond bThen bElse) t m l mc post
-    | if_false: forall t m l mc cond bThen bElse post,
-        eval_bcond l cond = Some false ->
-        exec bElse t m l
-             (addMetricLoads 2
-             (addMetricInstructions 2
-             (addMetricJumps 1 mc))) post ->
-        exec (SIf cond bThen bElse) t m l mc post
-    | loop: forall t m l mc cond body1 body2 mid1 mid2 post,
-        (* This case is carefully crafted in such a way that recursive uses of exec
-         only appear under forall and ->, but not under exists, /\, \/, to make sure the
-         auto-generated induction principle contains an IH for all recursive uses. *)
-        exec body1 t m l mc mid1 ->
-        (forall t' m' l' mc',
-            mid1 t' m' l' mc' ->
-            eval_bcond l' cond <> None) ->
-        (forall t' m' l' mc',
-            mid1 t' m' l' mc' ->
-            eval_bcond l' cond = Some false ->
-            post t' m' l'
-                 (addMetricLoads 1
-                 (addMetricInstructions 1
-                 (addMetricJumps 1 mc')))) ->
-        (forall t' m' l' mc',
-            mid1 t' m' l' mc' ->
-            eval_bcond l' cond = Some true ->
-            exec body2 t' m' l' mc' mid2) ->
-        (forall t'' m'' l'' mc'',
-            mid2 t'' m'' l'' mc'' ->
-            exec (SLoop body1 cond body2) t'' m'' l''
-                 (addMetricLoads 2
-                 (addMetricInstructions 2
-                 (addMetricJumps 1 mc''))) post) ->
-        exec (SLoop body1 cond body2) t m l mc post
-    | seq: forall t m l mc s1 s2 mid post,
-        exec s1 t m l mc mid ->
-        (forall t' m' l' mc', mid t' m' l' mc' -> exec s2 t' m' l' mc' post) ->
-        exec (SSeq s1 s2) t m l mc post
-    | skip: forall t m l mc post,
-        post t m l mc ->
-        exec SSkip t m l mc post
-*)
-.
-
-  End WithE.
-
-  Lemma mem_eq_trans: forall m1 m2 m3: option mem,
-      m1 == m2 -> m2 == m3 -> m1 == m3.
-  Admitted.
-
-  Lemma mem_eq_rewrite: forall F A L R: option mem,
-      L == R ->
-      A == L \+/ F ->
-      A == R \+/ F.
-  Admitted.
-
-  (* Note: does not hold if m is None! *)
-  Lemma mem_eq_refl: forall m A B: option mem,
-      A == B \+/ m -> (* <-- to assert that m is not None *)
-      m == m.
-  Proof.
-    unfold oeq, map.disj_putmany. intros. simp. clear. eauto.
-  Qed.
-
-  Section cancel_lemmas.
-    Let nth n xs := hd (@None mem) (skipn n xs).
-    Let remove_nth n (xs : list (option mem)) :=
-      (firstn n xs ++ tl (skipn n xs)).
-
-    Lemma mem_eq_cancel_at: forall (i j: nat) (xs ys: list (option mem)),
-        nth i xs = nth j ys ->
-        map.dus (remove_nth i xs) == map.dus (remove_nth j ys) ->
-        map.dus xs == map.dus ys.
-    Proof.
-    Admitted.
-  End cancel_lemmas.
-
-  Ltac cancel_at_indices i j :=
-    lazymatch goal with
-    | |- map.dus ?LHS == map.dus ?RHS =>
-      simple refine (mem_eq_cancel_at i j LHS RHS _ _);
-      cbn [firstn skipn List.app hd tl]
-    end.
+  Lemma sep_def: forall {m: mem} {P Q: mem -> Prop},
+      (P * Q)%sep m ->
+      exists m1 m2, map.split m m1 m2 /\ P m1 /\ Q m2.
+  Proof. unfold sep. intros *. apply id. Qed.
 
   Lemma spilling_correct (e e1 e2 : env) (Ev : envs_related e1 e2)
         (s1 : stmt)
   (t1 : trace)
-  (m1 : option mem)
-  (l1 : option locals)
+  (m1 : mem)
+  (l1 : locals)
   (mc1 : MetricLog)
-  (post : trace -> option mem -> option locals -> MetricLog -> Prop):
+  (post : trace -> mem -> locals -> MetricLog -> Prop):
   exec e1 s1 t1 m1 l1 mc1 post ->
-  forall (frame : option mem) (maxvar : Z),
+  forall (frame : mem -> Prop) (maxvar : Z),
   valid_vars_src maxvar s1 ->
-  forall (t2 : trace) (m2 : option mem) (l2 : option locals) (mc2 : MetricLog),
+  forall (t2 : trace) (m2 : mem) (l2 : locals) (mc2 : MetricLog),
   related maxvar frame false t1 m1 l1 mc1 t2 m2 l2 mc2 ->
   exec e2 (spill_stmt s1) t2 m2 l2 mc2
-    (fun (t2' : trace) (m2' : option mem) (l2' : option locals) (mc2' : MetricLog) =>
+    (fun (t2' : trace) (m2' : mem) (l2' : locals) (mc2' : MetricLog) =>
        exists t1' m1' l1' mc1',
          related maxvar frame false t1' m1' l1' mc1' t2' m2' l2' mc2' /\
          post t1' m1' l1' mc1').
   Proof.
     unfold related. induction 1; intros; simp; subst.
     - (* exec.interact *)
-      eapply interact.
-      + eapply mem_eq_trans. 1: eassumption.
-        eapply mem_eq_trans.
-        * eapply mem_eq_rewrite. 1: exact H.
-          match goal with
-          | |- ?L1 \+/ ?L2 \+/ ?L3 == ?R1 \+/ ?R2 =>
-            change (map.dus [L3; L2; L1] == map.dus [R2; R1])
-          end.
-          cancel_at_indices 2%nat 1%nat. 1: reflexivity.
-          cbv [map.dus].
-          eapply mem_eq_refl.
-          eapply mem_eq_trans. 1: exact H5p0.
-          match goal with
-          | |- ?L1 \+/ ?L2 \+/ ?L3 == ?R1 \+/ ?R2 =>
-            change (map.dus [L3; L2; L1] == map.dus [R2; R1])
-          end.
+      spec (subst_split (ok := mem_ok) m) as A.
+      1: eassumption. 1: ecancel_assumption.
+      edestruct (@sep_def m2 (eq mGive)) as (mGive' & mKeepL & B & ? & C).
+      1: simpl. (* PARAMRECORDS *) 1: ecancel_assumption.
+      subst mGive'.
+      simpl in H3. destruct H3 as [FR FA].
+      eapply map.getmany_of_list_to_split in H0.
+      destruct H0 as (l1rest & largs & F1 & S1).
+      (*unfold sep in H4p3. destruct H4p3 as (lRegs' & lStack' & S2 & ? & ?). subst lRegs' lStack'.*)
+      rename H4p3 into S2.
+      move S1 before S2. move FA after S2. move F1 before S1.
 
+      (* largs is contained in lRegs by FA, H4p0, H4p1
+         need interaction between map.dom and sep
 
-(*
-  Lemma spilling_sim(e1 e2: env):
-      envs_related e1 e2 ->
-      forall frame s1 maxvar,
-        valid_vars_src maxvar s1 ->
-        simulation (SimExec Z e1 s1) (SimExec Z e2 (spill_stmt s1))
-                   (related maxvar frame).
-  Proof.
-    unfold simulation, SimExec.
-    intros Ev frame s1 maxvar V (((t1 & m1) & l1) & mc1) (((t2 & m2) & l2) & mc2) post1 R Exec.
-    revert frame maxvar V t2 m2 l2 mc2 R.
-    unfold compile_inv, related.
-    match type of Exec with
-    | FlatImp.exec _ _ _ _ _ _ ?P => remember P as post
-    end.
-    revert post1 Heqpost.
-    induction Exec; simpl; intros; simp; subst.
-    - (* exec.interact *)
+      eapply @exec.interact with (mGive := mGive).
+      + eapply map.split_comm. exact B.
+      +
 
-
-    - (* exec.interact *)
-      eapply map.split_splits in H.
-      eapply @exec.interact with (mGive := mGive) (mKeep := map.putmany mKeep (map.putmany mStack frame)).
-      + eapply map.splits_split.
-
-(*
-
-disjoint union on "option map" ?
-m \+/ mStack \+/ frame
-
-lRegs \+/ tmp1 ~> tmp1val \+/ tmp2 ~> tmp2val
-
-but what to pass to exec.interact? -> also "option map"
-
-disjoint_putmany
-
-just congruence:
-a = c ->
-b = d ->
-a \+/ b = c \+/ d
-
-*)
-      + unfold map.split in *; simp. split.
-        * remember (map.putmany mStack frame) as A.
-          rewrite <- map.putmany_assoc.
-          { erewrite <- (@map.putmany_assoc _ _ _ _ _ word.eqb_spec).
-            { f_equal.
-              apply map.putmany_comm.
-              subst A.
-
-          1: exact mem_ok.
-
-          { assert (map.ok FlatImp.mem = map.ok mem). {
-              clear.
-              reflexivity.
-
-rewrite <- (@map.putmany_assoc _ _ _ mem_ok word.eqb).
-
-
-subst. eapply split_interact; try eassumption.
       + erewrite map__getmany_of_list_shrink. 2: eassumption. 2: {
           eapply Forall_impl. 2: eassumption.
           clear -localsOk. unfold fp, tmp1, tmp2. intros.
@@ -888,173 +497,22 @@ subst. eapply split_interact; try eassumption.
         }
         admit. (* ok, but TODO use map__dom instead of map__dom_in *)
 
-    - (* exec.call *)
-      admit.
-    - (* exec.load *)
-      eapply seq_cps.
-      unfold load_arg_reg1, arg_reg1, save_res_reg, res_reg, stack_loc.
-      destr (Z.leb 32 a).
-      + match goal with
-        | H: spilled_vars _ _ _ _ |- _ => pose proof H as A
-        end.
-        unfold spilled_vars in A.
-        assert (32 <= a <= maxvar) as B by blia. specialize A with (1 := B); clear B. simp.
-        eapply exec.load with (addr0 := fpval) (v1 := v0).
-        * admit. (* ok *)
-        * eapply grow_load. 1: eassumption.
-
-jj
-admit. (* growing from mStack to m2 preserves Memory.load *)
-        * eapply seq_cps. eapply exec.load. {
-            rewrite map.get_put_same. reflexivity.
-          } {
-            match goal with
-            | |- _ = ?opt => unify opt (Some v)
-            end.
-            assert (map.get lStack a = Some addr) as B by admit.
-            specialize Ar with (1 := B). subst v0.
-            (* growing from m to m2 preserves Memory.load *)
-            admit.
-          } {
-            destr (Z.leb 32 x).
-            - eapply exec.store.
-              + rewrite ?map.get_put_diff by (cbv; discriminate).
-                match goal with
-                | |- _ = ?opt => unify opt (Some fpval)
-                end.
-                admit. (* ok *)
-              + rewrite map.get_put_same. reflexivity.
-              + admit. (* memory stuff... *)
-              + repeat match goal with
-                       | |- exists (_: FlatImp.SimState _), _ => refine (ex_intro _ (_, _, _, _) _)
-                       | |- exists _, _ => eexists
-                       | |- _ /\ _ => split
-                       end.
-                1: reflexivity.
-                8: eassumption.
-                * admit.
-                * admit.
-                * admit.
-                * admit.
-                * admit.
-                * rewrite map.put_put_same. admit.
-                * admit.
-            - admit.
-          }
-      + admit.
-    - (* exec.store *)
-      admit.
-    - (* exec.stackalloc *)
-      rename H1 into IH.
-      unfold save_res_reg, res_reg, stack_loc.
-      destr (Z.leb 32 x).
-      + eapply exec.stackalloc. 1: assumption.
-        intros. eapply seq_cps. eapply exec.store.
-        * rewrite map.get_put_diff by discriminate.
+      + eapply mem_eq_trans. 1: eassumption.
+        eapply mem_eq_trans.
+        * eapply mem_eq_rewrite. 1: exact H.
           match goal with
-          | |- _ = ?opt => unify opt (Some fpval)
+          | |- ?L1 \+/ ?L2 \+/ ?L3 == ?R1 \+/ ?R2 =>
+            change (map.dus [L3; L2; L1] == map.dus [R2; R1])
           end.
-          admit. (* ok *)
-        * rewrite map.get_put_same. reflexivity.
-        * unfold Memory.store, Memory.store_Z, Memory.store_bytes.
-          destruct_one_match. 2: admit. (* shouldn't happen *)
-          reflexivity.
-        * eapply exec.weaken. {
-            pose (fun m => (Memory.unchecked_store_bytes (Memory.bytes_per Syntax.access_size.word) m
-                      (word.add fpval (word.of_Z ((x - 32) * bytes_per_word)))
-            (LittleEndian.split (@Memory.bytes_per width Syntax.access_size.word) (word.unsigned a)))) as upd.
-            match goal with
-            | |- exec _ _ _ ?M _ _ _ => change M with (upd mCombined)
-            end.
-            rename mStack0 into mStackHL.
-            (* mStack is our stack memory used for spilling, while mStackHL is allocated by this
-               SStackalloc and exposed as memory to the source program *)
-            eapply IH with (mCombined := map.putmany mSmall mStackHL) (frame := frame)
-                           (post2 := fun '(t', m', l', mc') =>
-                                       exists mSmall' mStack',
-                                         Memory.anybytes a n mStack' /\ map.split m' mSmall' mStack' /\
-                                         post1 (t', mSmall', l', mc')).
-            1: eassumption.
-            1: eapply split_stackalloc_1; eassumption.
-            1: reflexivity.
-            1: eassumption.
-            (* existentials to pick to satisfy relation before invoking IH *)
-            eexists fpval, a, tmp2val, (upd mL), (upd mStack), (map.put lStack x a), lRegs.
-            ssplit.
-            1: reflexivity.
-            1: {
-              eapply split_stackalloc_2 with (m3 := upd m2). 1,2: admit. (* ok *)
-            }
-            1: admit. (* ok *)
-            1: eassumption.
-            1: eapply map__dom_in_put; [assumption|blia].
-            1: admit. (* ok *)
-            1: admit. (* ok *)
-            1: admit. (* ok *)
-          }
-          simpl. intros. simp.
-          exists (map.putmany mSmall' mL0), mStack'.
-          repeat match goal with
-                 | |- exists (_: FlatImp.SimState _), _ => refine (ex_intro _ (_, _, _, _) _)
-                 | |- exists _, _ => eexists
-                 | |- _ /\ _ => split
-                 end.
-          11: eassumption.
-          1: eassumption.
-          1: eapply split_stackalloc_2; eassumption.
-          1: reflexivity.
-          1: {
-            match goal with
-            | |- map.split _ _ ?M => unify M mL0
-            end.
-            eapply split_stackalloc_1; eassumption.
-          }
-          1: eassumption.
-          5: eassumption.
-          all: try eassumption.
-      + admit. (* same but without spilling *)
-    - (* exec.lit *)
-      admit.
-    - (* exec.op *)
-      admit.
-    - (* exec.set *)
-      admit.
-    - (* exec.if_true *)
-      unfold prepare_bcond. destruct cond.
-      + simpl. eapply seq_cps. eapply seq_cps. simpl in *. simp.
-        unfold load_arg_reg1, arg_reg1, load_arg_reg2, arg_reg2, save_res_reg, res_reg, stack_loc.
-        destr (Z.leb 32 x).
-        * match goal with
-          | H: spilled_vars _ _ _ _ |- _ => pose proof H as A
+          cancel_at_indices 2%nat 1%nat. 1: reflexivity.
+          cbv [map.dus].
+          eapply mem_eq_refl.
+          eapply mem_eq_trans. 1: exact H5p0.
+          match goal with
+          | |- ?L1 \+/ ?L2 \+/ ?L3 == ?R1 \+/ ?R2 =>
+            change (map.dus [L3; L2; L1] == map.dus [R2; R1])
           end.
-          unfold spilled_vars in A.
-          assert (32 <= x <= maxvar) as B by blia.
-          specialize A with (1 := B); clear B. simp.
-          eapply exec.load with (addr := fpval).
-          { admit. }
-          {
-
-
-            Search Memory.load map.split.
-
-exact Al. eassumption. }
-
-            match goal with
-          | H: spilled_vars _ _ _ _ |- _ => pose proof H as A
-          end.
-          unfold spilled_vars in A.
-          assert (32 <= a <= maxvar) as B by blia. specialize A with (1 := B); clear B. simp.
-          eapply exec.load with (addr0 := fpval) (v1 := v0).
-        * admit. (* ok *)
-
-
-    - (* exec.if_false *)
-    - (* exec.loop *)
-    - (* exec.seq *)
-    - (* exec.skip *)
 *)
-
-
   Abort.
 
 End Spilling.
